common/LanguageInterface.v
@@ -58,77 +58,62 @@ Definition li_wp :=
 Record callconv {li1 li2} :=
   mk_callconv {
     ccworld : Type;
-    valid_skel sk1 sk2: Genv.skel_path sk1 sk2 -> Prop;
-    match_senv:
-        ccworld -> forall sk1 sk2, Genv.skel_path sk1 sk2 ->
-        Genv.symtbl -> Genv.symtbl -> Prop;
+    valid_skel (removed: Genv.removed_symbols)
+      (sk1 sk2: AST.program unit unit): Prop;
+    match_senv (removed: Genv.removed_symbols):
+        ccworld -> Genv.symtbl -> Genv.symtbl -> Prop;
     match_query: ccworld -> query li1 -> query li2 -> Prop;
     match_reply: ccworld -> reply li1 -> reply li2 -> Prop;
-
-    match_senv_local:
-    forall sk1 sk2 w path se1 se2,
-      valid_skel _ _ path ->
-      match_senv w sk1 sk2 path se1 se2 ->
-      Genv.valid_stbls' sk1 sk2 se1 se2;
   }.
 
 Arguments callconv: clear implicits.
-Arguments match_senv {_ _} _ _ {_ _} _.
-Arguments valid_skel {_ _} _ {_ _} _.
 Delimit Scope cc_scope with cc.
 Bind Scope cc_scope with callconv.
 Local Obligation Tactic := cbn; eauto.
 
 (** ** Identity *)
 
-Definition valid_skel_id {sk1 sk2} (path: Genv.skel_path sk1 sk2) : Prop.
-Proof.
-  destruct path.
-  - refine True.
-  - refine False.
-  - refine False.
-Defined.
+Inductive valid_skel_id:
+    Genv.removed_symbols -> AST.program unit unit -> AST.program unit unit -> Prop :=
+| valid_skel_id_intro sk:
+    valid_skel_id (Genv.Removed (fun id => False)) sk sk.
 
 Program Definition cc_id {li}: callconv li li :=
   {|
     ccworld := unit;
-    valid_skel sk1 sk2 sk_path := valid_skel_id sk_path;
-    match_senv w _ _ _ se1 se2 := se1 = se2;
+    valid_skel := valid_skel_id;
+    match_senv w _ se1 se2 := se1 = se2;
     match_query w := eq;
     match_reply w := eq;
   |}.
-Next Obligation.
-  intros. subst.
-  (* FIXME: we need some [Genv.valid_for] in [match_senv] *)
-Admitted.
 
 Notation "1" := cc_id : cc_scope.
 
 (** ** Composition *)
 
 Inductive valid_skel_compose {li1 li2 li3} (cc12: callconv li1 li2)
-  (cc23: callconv li2 li3) sk1 sk3: Genv.skel_path sk1 sk3 -> Prop :=
-  | Valid_skel_compose_intro sk2 (path12: Genv.skel_path sk1 sk2)
-      (path23: Genv.skel_path sk2 sk3):
-      valid_skel cc12 path12 -> valid_skel cc23 path23 ->
-      valid_skel_compose cc12 cc23 _ _ (Genv.Compose path12 path23).
+  (cc23: callconv li2 li3):
+    Genv.removed_symbols -> AST.program unit unit -> AST.program unit unit -> Prop :=
+  | Valid_skel_compose_intro removed1 removed2 sk1 sk2 sk3:
+      valid_skel cc12 removed1 sk1 sk2 ->
+      valid_skel cc23 removed2 sk2 sk3 ->
+      valid_skel_compose cc12 cc23 (Genv.Compose removed1 removed2) sk1 sk3.
 
-Inductive match_senv_compose
-  {li1 li2 li3} (cc12: callconv li1 li2) (cc23: callconv li2 li3):
-  Genv.symtbl * ccworld cc12 * ccworld cc23 ->
-  forall sk1 sk3, Genv.skel_path sk1 sk3 -> Genv.symtbl -> Genv.symtbl -> Prop :=
-  | Match_senv_compose_intro se1 se2 se3 sk1 sk2 sk3 w12 w23
-      (path12: Genv.skel_path sk1 sk2) (path23: Genv.skel_path sk2 sk3)
-      (SE12: match_senv cc12 w12 path12 se1 se2)
-      (SE23: match_senv cc23 w23 path23 se2 se3):
-      match_senv_compose cc12 cc23 (se2, w12, w23)
-        sk1 sk3 (Genv.Compose path12 path23) se1 se3.
+Inductive match_senv_compose {li1 li2 li3} (cc12: callconv li1 li2)
+  (cc23: callconv li2 li3):
+    Genv.removed_symbols -> (Genv.symtbl * ccworld cc12 * ccworld cc23) ->
+    Genv.symtbl -> Genv.symtbl -> Prop :=
+  | Match_senv_compose_intro removed1 removed2 w12 w23 se1 se2 se3:
+      match_senv cc12 removed1 w12 se1 se2 ->
+      match_senv cc23 removed2 w23 se2 se3 ->
+      match_senv_compose cc12 cc23 (Genv.Compose removed1 removed2)
+        (se2, w12, w23) se1 se3.
 
 Program Definition cc_compose {li1 li2 li3} (cc12: callconv li1 li2) (cc23: callconv li2 li3) :=
   {|
     ccworld := Genv.symtbl * ccworld cc12 * ccworld cc23;
     valid_skel := valid_skel_compose cc12 cc23;
-    match_senv w := match_senv_compose cc12 cc23 w;
+    match_senv := match_senv_compose cc12 cc23;
     match_query '(se2, w12, w23) q1 q3 :=
       exists q2,
         match_query cc12 w12 q1 q2 /\
@@ -138,14 +123,6 @@ Program Definition cc_compose {li1 li2 li3} (cc12: callconv li1 li2) (cc23: call
         match_reply cc12 w12 r1 r2 /\
         match_reply cc23 w23 r2 r3;
   |}.
-Next Obligation.
-  intros. rename sk2 into sk3. rename se2 into se3.
-  destruct w as [[se2 w12] w23]. inv H. inv H0.
-  subst_dep.
-  apply match_senv_local in SE12; eauto.
-  apply match_senv_local in SE23; eauto.
-  eapply Genv.valid_stbls'_compose; eauto.
-Qed.
 
 Infix "@" := cc_compose (at level 30, right associativity) : cc_scope.
 
@@ -199,12 +176,14 @@ Inductive cc_c_reply R (w: world R): relation c_reply :=
 
 (* TODO: for most passes we use [valid_skel_id], but for Unusedglob, we need
    something more general *)
-Program Definition cc_c (R: cklr): callconv li_c li_c :=
-  {|
-    ccworld := world R;
-    valid_skel _ _ path := valid_skel_id path;
-    match_senv w sk1 sk2 _sk_path se1 se2 :=
-      match_stbls R w se1 se2 /\ Genv.valid_stbls' sk1 sk2 se1 se2;
-    match_query := cc_c_query R;
-    match_reply := (<> cc_c_reply R)%klr;
-  |}.
+
+
+(* Program Definition cc_c (R: cklr): callconv li_c li_c := *)
+(*   {| *)
+(*     ccworld := world R; *)
+(*     valid_skel := valid_skel_id; *)
+(*     match_senv w removed se1 se2 := *)
+(*       match_stbls R w se1 se2 /\ Genv.valid_stbls' sk1 sk2 se1 se2; *)
+(*     match_query := cc_c_query R; *)
+(*     match_reply := (<> cc_c_reply R)%klr; *)
+(*   |}. *)
