common/Smallstep.v
@@ -549,9 +549,9 @@ Record fsim_properties (L1: lts liA1 liB1 state1) (L2: lts liA2 liB2 state2) (in
        way horizontal composition doesn't work *)
     fsim_match_external:
       forall i s1 s2 q1, match_states i s1 s2 -> at_external L1 s1 q1 ->
-      forall sk1 sk2 (path: Genv.skel_path sk1 sk2), valid_skel ccA path ->
+      forall sk1 sk2 (removed: Genv.removed_symbols), valid_skel ccA removed sk1 sk2 ->
       exists w q2, at_external L2 s2 q2 /\ match_query ccA w q1 q2 /\
-      match_senv ccA w path se1 se2 /\
+      match_senv ccA removed w se1 se2 /\
       forall r1 r2 s1', match_reply ccA w r1 r2 -> after_external L1 s1 r1 s1' ->
       exists i' s2', after_external L2 s2 r2 s2' /\ match_states i' s1' s2';
     fsim_simulation:
@@ -606,9 +606,9 @@ Hypothesis match_final_states:
 
 Hypothesis match_external:
   forall s1 s2 q1, match_states s1 s2 -> at_external L1 s1 q1 ->
-  forall sk1 sk2 (path: Genv.skel_path sk1 sk2), valid_skel ccA path ->
+  forall sk1 sk2 (removed: Genv.removed_symbols), valid_skel ccA removed sk1 sk2 ->
   exists wA q2, at_external L2 s2 q2 /\ match_query ccA wA q1 q2 /\
-  match_senv ccA wA path se1 se2 /\
+  match_senv ccA removed wA se1 se2 /\
   forall r1 r2 s1', match_reply ccA wA r1 r2 -> after_external L1 s1 r1 s1' ->
   exists s2', after_external L2 s2 r2 s2' /\ match_states s1' s2'.
 
@@ -829,12 +829,11 @@ Record fsim_components {liA1 liA2} (ccA: callconv liA1 liA2)
     fsim_order: fsim_index -> fsim_index -> Prop;
     fsim_match_states: _;
 
-    fsim_skel:
-      Genv.skel_path (skel L1) (skel L2);
+    fsim_removed: Genv.removed_symbols;
     fsim_skel_valid:
-      valid_skel ccB fsim_skel;
+      valid_skel ccB fsim_removed (skel L1) (skel L2);
     fsim_lts se1 se2 wB:
-      match_senv ccB wB fsim_skel se1 se2 ->
+      match_senv ccB fsim_removed wB se1 se2 ->
       fsim_properties ccA ccB se1 se2 wB (activate L1 se1) (activate L2 se2)
         fsim_index fsim_order (fsim_match_states se1 se2 wB);
     fsim_order_wf:
@@ -887,7 +886,7 @@ Proof.
   (* eapply Forward_simulation. *)
   (* instantiate (1 := (fun _ _ _ => _)). *)
   eapply Forward_simulation with
-    _ (fun _ _ _ _ => _) (Genv.Same (skel L)); auto.
+    _ (fun _ _ _ _ => _) (Genv.Removed (fun _ => False)); auto.
   - econstructor.
   - intros se ? w Hse. inv Hse. destruct w.
     eapply forward_simulation_plus with (match_states := eq);
@@ -928,14 +927,12 @@ Proof.
   (* destruct H12 as [index order match_states path12 props order_wf] eqn: Hf12. *)
   (* destruct H23 as [index' order' match_states' path23 props' order_wf'] eqn: Hf23. *)
   apply Forward_simulation
-    with ff_order ff_match_states (Genv.Compose (fsim_skel H12) (fsim_skel H23)).
-  { constructor. apply H12. apply H23. }
+    with ff_order ff_match_states (Genv.Compose (fsim_removed H12) (fsim_removed H23)).
+  { econstructor. apply H12. apply H23. }
   2: { unfold ff_order. destruct H12. destruct H23.
        auto using wf_lex_ord, wf_clos_trans. }
   intros se1 se3 [[se2 w] w'] Hse. cbn in *.
-  inv Hse. subst_dep.
-  pose proof (fsim_lts H12) as props.
-  pose proof (fsim_lts H23) as props'.
+  inv Hse. pose proof (fsim_lts H12) as props. pose proof (fsim_lts H23) as props'.
 
   constructor.
 - (* valid_query *)
