common/SmallstepLinking.v
@@ -177,13 +177,14 @@ Section FSIM.
   Context (L2 : I -> Smallstep.semantics li2 li2).
   Context (HL : forall i, fsim_components cc cc (L1 i) (L2 i)).
   Context (se1 se2: Genv.symtbl) (w : ccworld cc).
-  Context (Hse: forall i, match_senv cc w (fsim_skel (HL i)) se1 se2).
-  Context (Hvs : forall i : I, valid_skel cc (fsim_skel (HL i))).
+  Context (Hse: forall i, match_senv cc (fsim_removed (HL i)) w se1 se2).
+  Context (sk1i sk2i: forall (i: I), AST.program unit unit).
+  Context (Hsk: forall i, valid_skel cc (fsim_removed (HL i)) (sk1i i) (sk2i i)).
   Notation index := {i & fsim_index (HL i)}.
 
   Inductive match_topframes wk: index -> frame L1 -> frame L2 -> Prop :=
     match_topframes_intro i s1 s2 idx:
-      match_senv cc wk (fsim_skel (HL i)) se1 se2 ->
+      match_senv cc (fsim_removed (HL i)) wk se1 se2 ->
       fsim_match_states (HL i) se1 se2 wk idx s1 s2 ->
       match_topframes wk
         (existT _ i idx)
@@ -192,7 +193,7 @@ Section FSIM.
 
   Inductive match_contframes wk wk': frame L1 -> frame L2 -> Prop :=
     match_contframes_intro i s1 s2:
-      match_senv cc wk' (fsim_skel (HL i)) se1 se2 ->
+      match_senv cc (fsim_removed (HL i)) wk' se1 se2 ->
       (forall r1 r2 s1', match_reply cc wk r1 r2 ->
        Smallstep.after_external (L1 i se1) s1 r1 s1' ->
        exists idx s2',
@@ -283,20 +284,25 @@ Section FSIM.
 
   Lemma external_simulation:
     forall idx s1 s2 qx1, match_states idx s1 s2 -> at_external L1 se1 s1 qx1 ->
-    forall sk1 sk2 (path: Genv.skel_path sk1 sk2), valid_skel cc path ->
+    forall sk1 sk2 (removed: Genv.removed_symbols), valid_skel cc removed sk1 sk2 ->
     exists wx qx2, at_external L2 se2 s2 qx2 /\  match_query cc wx qx1 qx2 /\
-    match_senv cc wx path se1 se2 /\
+    match_senv cc removed wx se1 se2 /\
     forall rx1 rx2 s1', match_reply cc wx rx1 rx2 -> after_external L1 se1 s1 rx1 s1' ->
     exists idx' s2', after_external L2 se2 s2 rx2 s2' /\ match_states idx' s1' s2'.
   Proof.
-    intros idx s1 s2 q1 Hs Hq1 sk1 sk2 path Hpath.
+    intros idx s1 s2 q1 Hs Hq1 sk1' sk2' rem Hrem.
     destruct Hq1 as [i s1 qx1 k1 Hqx1 Hvld].
     inv Hs. inv H2. subst_dep. clear idx0.
     pose proof (fsim_lts (HL i) _ _ _ H3) as Hi.
     edestruct @fsim_match_external as (wx & qx2 & Hqx2 & Hqx & Hsex & H); eauto.
     exists wx, qx2. intuition idtac.
     + constructor. eauto. intros j.
-      (* XXX: I suspect this could be fixed by footprint *)
+      erewrite fsim_match_valid_query; eauto.
+      apply HL.
+      (* XXX: I suspect this could be fixed by the [footprint] version of
+         forward simulation. [valid_query] may not be same, but at least when
+         [valid_query (L1 j) q = false], we have [valid_query (L2 j) q =
+         false] *)
       admit.
     + inv H1; subst_dep.
       edestruct H as (idx' & s2' & Hs2' & Hs'); eauto.
@@ -329,29 +335,19 @@ Definition compose {li} (La Lb: Smallstep.semantics li li) :=
   let L i := match i with true => La | false => Lb end in
   option_map (semantics L) (link (skel La) (skel Lb)).
 
-Record packed_path: Type := {
-    src_skel: AST.program unit unit;
-    tgt_skel: AST.program unit unit;
-    skel_path: Genv.skel_path src_skel tgt_skel;
-  }.
-
-Fixpoint compose_path {sk1a sk2a sk1b sk2b}
-                      (patha: Genv.skel_path sk1a sk2a)
-                      (pathb: Genv.skel_path sk1b sk2b): option packed_path.
-Proof.
-  destruct patha eqn: HA; destruct pathb eqn: Hb.
-  - destruct (link t t0) eqn: Hlink.
-    + refine (Some {| src_skel := p; tgt_skel := p; skel_path := Genv.Same p |}).
-    + refine None.
-  (* we could also combine [Same] and [Direct] *)
-  - refine None.
-  - refine None.
-  - refine None.
-  - destruct (link start start0) eqn: Hlink1.
-    + destruct (link end_ end_0) eqn: Hlink2.
+Lemma compose_removed {li1 li2} (cc: callconv li1 li2)
+  removed1 removed2 sk1l sk1r sk2l sk2r sk1 sk2:
+  valid_skel cc removed1 sk1l sk2l ->
+  valid_skel cc removed2 sk1r sk2r ->
+  link sk1l sk1r = Some sk1 ->
+  link sk2l sk2r = Some sk2 ->
+  exists removed,
+    valid_skel cc removed sk1 sk2 /\
+    forall se1 se2 w,
+      match_senv cc removed w se1 se2 ->
+      match_senv cc removed1 w se1 se2 /\
+      match_senv cc removed2 w se1 se2.
 Admitted.
-
-(* TODO: compose paths *)
 
 Lemma compose_simulation {li1 li2} (cc: callconv li1 li2) L1a L1b L1 L2a L2b L2:
   forward_simulation cc cc L1a L2a ->
@@ -365,20 +361,20 @@ Proof.
   destruct (link (skel L2a) (skel L2b)) as [sk2|] eqn:Hsk2; try discriminate. inv H2.
   set (L1 := fun i:bool => if i then L1a else L1b).
   set (L2 := fun i:bool => if i then L2a else L2b).
+  set (sk1i := fun i:bool => if i then (skel L1a) else (skel L1b)).
+  set (sk2i := fun i:bool => if i then (skel L2a) else (skel L2b)).
   assert (HL: forall i, fsim_components cc cc (L1 i) (L2 i)) by (intros [|]; auto).
+  edestruct (compose_removed cc) as (removed & Hsk & HSE).
+  apply (HL true). apply (HL false). 1-2: eauto.
   constructor.
-  eapply Forward_simulation with
-    (order cc L1 L2 HL) (match_states cc L1 L2 HL)
-    (path_compose (fsim_skel Ha) (fsim_skel Hb) Hsk1 Hsk2).
-  - destruct Ha, Hb. cbn. congruence.
-  - intros se1 se2 w Hse Hse1.
-    eapply semantics_simulation; eauto.
-    pose proof (link_linkorder _ _ _ Hsk1) as [Hsk1a Hsk1b].
-    intros [|]; cbn; eapply Genv.valid_for_linkorder; eauto.
+  eapply Forward_simulation with (order cc L1 L2 HL) (match_states cc L1 L2 HL) removed.
+  - apply Hsk.
+  - intros se1 se2 w Hse.
+    eapply semantics_simulation with sk1i sk2i.
+    + specialize (HSE _ _ _ Hse) as (? & ?).
+      intros [|]; eauto.
+    + intros [|]; eauto. apply (HL true). apply (HL false).
   - clear - HL. intros [i x].
     induction (fsim_order_wf (HL i) x) as [x Hx IHx].
     constructor. intros z Hxz. inv Hxz; subst_dep. eauto.
-  - intros. unfold valid_query. f_equal.
-    + eapply (fsim_lts (HL true)); eauto.
-    + eapply (fsim_lts (HL false)); eauto.
 Qed.
